#+Title: Logic and Proof
#+Author: [[http://www.andrew.cmu.edu/user/avigad][Jeremy Avigad]], [[http://www.andrew.cmu.edu/user/rlewis1/][Robert Y. Lewis]],  [[http://www.contrib.andrew.cmu.edu/~fpv/][Floris van Doorn]]

* Natural Deduction Rules

*** Implication

\begin{quote}
\AXM{}
\RLM{a}
\UIM{A}
\noLine
\UIM{\vdots}
\noLine
\UIM{B}
\RLM{a \;\; \mathord{\to}\mathrm{I}}
\UIM{A \to B}
\DP
\quad\quad
\AXM{A \to B}
\AXM{A}
\RLM{\mathord{\to}\mathrm{E}}
\BIM{B}
\DP
\end{quote}

*** Conjunction

\begin{quote}
\AXM{A}
\AXM{B}
\RLM{\mathord{\wedge}\mathrm{I}}
\BIM{A \wedge B}
\DP
\quad\quad
\AXM{A \wedge B}
\RLM{\mathord{\land}\mathrm{E_l}}
\UIM{A}
\DP
\quad\quad
\AXM{A \wedge B}
\RLM{\mathord{\land}\mathrm{E_r}}
\UIM{B}
\DP
\end{quote}

*** Negation

\begin{quote}
\AXM{}
\RLM{a}
\UIM{A}
\noLine
\UIM{\vdots}
\noLine
\UIM{\bot}
\RLM{a \;\; \lnot \mathrm{I}}
\UIM{\lnot A}
\DP
\quad\quad
\AXM{\lnot A}
\AXM{A}
\RLM{\lnot \mathrm{E}}
\BIM{\bot}
\DP
\end{quote}

*** Disjunction

\begin{quote}
\AXM{A}
\RLM{\mathord{\lor}\mathrm{I_l}}
\UIM{A \lor B}
\DP
\quad\quad
\AXM{B}
\RLM{\mathord{\lor}\mathrm{I_r}}
\UIM{A \lor B}
\DP
\quad\quad
\AXM{A \vee B}
\AXM{}
\RLM{a}
\UIM{A}
\noLine
\UIM{\vdots}
\noLine
\UIM{C}
\AXM{}
\RLM{b}
\UIM{B}
\noLine
\UIM{\vdots}
\noLine
\UIM{C}
\RLM{a, b \;\; \mathord{\lor}\mathrm{E}}
\TIM{C}
\DP
\end{quote}

*** Truth and falsity

\begin{quote}
\AXM{\bot}
\RLM{\bot \mathrm{E}}
\UIM{A}
\DP
\quad\quad
\AXM{}
\RLM{\top \mathrm{I}}
\UIM{\top}
\DP
\end{quote}


*** Bi-implication

\begin{quote}
\AXM{}
\RLM{a}
\UIM{A}
\noLine
\UIM{\vdots}
\noLine
\UIM{B}
\AXM{}
\RLM{b}
\UIM{B}
\noLine
\UIM{\vdots}
\noLine
\UIM{A}
\RLM{a, b \;\; \mathord{\liff}\mathrm{I}}
\BIM{A \liff B}
\DP
\AXM{A \liff B}
\AXM{A}
\RLM{\mathord{\liff}\mathrm{E}_l}
\BIM{B}
\DP
\quad\quad
\AXM{A \liff B}
\AXM{B}
\RLM{\mathord{\liff}\mathrm{E}_r}
\BIM{A}
\DP
\end{quote}

*** Reductio ad absurdum (proof by contradiction)

\begin{quote}
\AXM{}
\RLM{a}
\UIM{\neg A}
\noLine
\UIM{\vdots}
\noLine
\UIM{\bot}
\RLM{a \;\; \mathrm{RAA}}
\UIM{A}
\DP
\end{quote}

*** Universal quantifier

\begin{quote}
\AXM{A(x)}
\RLM{\mathord{\forall}\mathrm{I}}
\UIM{\fa y A(y)}
\DP
\quad\quad
\AXM{\fa x A(x)}
\RLM{\mathord{\forall}\mathrm{E}}
\UIM{A(t)}
\DP
\end{quote}
In the introduction rule, $x$ should not be free in any uncanceled
hypothesis. In the elimination rule, $t$ can be any term that does not
clash with any of the bound variables in $A$.

*** Existential quantifier

\begin{quote}
\AXM{A(t)}
\RLM{\mathord{\exists}\mathrm{I}}
\UIM{\ex x A(x)}
\DP
\quad\quad
\AXM{\ex x A(x)}
\AXM{}
\RLM{a}
\UIM{A(y)}
\noLine
\UIM{\vdots}
\noLine
\UIM{B}
\RLM{a \;\; \mathord{\exists}\mathrm{E}}
\BIM{B}
\DP
\end{quote}
In the introduction rule, $t$ cant be any term that does not clash
with any of the bound variables in $A$. In the elimination rule, $y$
should not be free in $B$ or any uncanceled hypothesis.

*** Equality

\begin{center}
\AXM{}
\RLM{\mathrm{refl}}
\UIM{t = t}
\DP
\quad
\AXM{s = t}
\RLM{\mathrm{symm}}
\UIM{t = s}
\DP
\quad
\AXM{r = s}
\AXM{s = t}
\RLM{\mathrm{trans}}
\BIM{r = t}
\DP
\\
\ \\
\AXM{s = t}
\RLM{\mathrm{subst}}
\UIM{r(s) = r(t)}
\DP
\quad
\AXM{s = t}
\RLM{\mathrm{subst}}
\AXM{P(s)}
\BIM{P(t)}
\DP
\end{center}
Strictly speaking, only $\mathrm{refl}$ and the second substitution
rule are necessary. The others can be derived from them.

